feat: Add branch key id supplier for hierarchical keyring (#150)

AwsCryptographicMaterialProviders/runtimes/java/src/main/smithy-generated/software/amazon/cryptography/materialProviders/IBranchKeyIdSupplier.java
@@ -1,0 +1,11 @@
+// Copyright Amazon.com Inc. or its affiliates. All Rights Reserved.
+// SPDX-License-Identifier: Apache-2.0
+// Do not modify this file. This file is machine generated, and any changes to it will be overwritten.
+package software.amazon.cryptography.materialProviders;
+
+import software.amazon.cryptography.materialProviders.model.GetBranchKeyIdInput;
+import software.amazon.cryptography.materialProviders.model.GetBranchKeyIdOutput;
+
+public interface IBranchKeyIdSupplier {
+  GetBranchKeyIdOutput GetBranchKeyId(GetBranchKeyIdInput nativeValue);
+}
