AwsCryptographicMaterialProviders/runtimes/net/Generated/BranchKeyIdSupplier.cs
@@ -1,0 +1,23 @@
+// Copyright Amazon.com Inc. or its affiliates. All Rights Reserved.
+// SPDX-License-Identifier: Apache-2.0
+// Do not modify this file. This file is machine generated, and any changes to it will be overwritten.
+using System;
+using System.IO;
+using System.Collections.Generic;
+using AWS.Cryptography.MaterialProviders;
+using Dafny.Aws.Cryptography.MaterialProviders.Types;
+namespace AWS.Cryptography.MaterialProviders
+{
+  internal class BranchKeyIdSupplier : BranchKeyIdSupplierBase
+  {
+    internal readonly Dafny.Aws.Cryptography.MaterialProviders.Types.IBranchKeyIdSupplier _impl;
+    internal BranchKeyIdSupplier(Dafny.Aws.Cryptography.MaterialProviders.Types.IBranchKeyIdSupplier impl) { this._impl = impl; }
+    protected override AWS.Cryptography.MaterialProviders.GetBranchKeyIdOutput _GetBranchKeyId(AWS.Cryptography.MaterialProviders.GetBranchKeyIdInput input)
+    {
+      Dafny.Aws.Cryptography.MaterialProviders.Types._IGetBranchKeyIdInput internalInput = TypeConversion.ToDafny_N3_aws__N12_cryptography__N17_materialProviders__S19_GetBranchKeyIdInput(input);
+      Wrappers_Compile._IResult<Dafny.Aws.Cryptography.MaterialProviders.Types._IGetBranchKeyIdOutput, Dafny.Aws.Cryptography.MaterialProviders.Types._IError> result = this._impl.GetBranchKeyId(internalInput);
+      if (result.is_Failure) throw TypeConversion.FromDafny_CommonError(result.dtor_error);
+      return TypeConversion.FromDafny_N3_aws__N12_cryptography__N17_materialProviders__S20_GetBranchKeyIdOutput(result.dtor_value);
+    }
+  }
+}
