AwsCryptographicMaterialProviders/test/Keyrings/AwsKms/AwsKmsHierarchicalKeyring/TestAwsKmsHierarchicalKeyring.dfy
@@ -27,6 +27,17 @@ module TestAwsKmsHierarchicalKeyring {
   const keyArn := "arn:aws:kms:us-west-2:370957321024:key/9d989aa2-2f9c-438c-a745-cc57d3ad0126";
   const branchKeyStoreArn := "arn:aws:dynamodb:us-west-2:370957321024:table/HierarchicalKeyringTestTable";
 
+  // These tests require a keystore populated with these keys
+  const BRANCH_KEY_ID := "hierarchy-test-v1";
+  const ACTIVE_ACTIVE_BRANCH_KEY_ID := "hierarchy-test-active-active";
+
+  // Constants for TestBranchKeySupplier
+  const BRANCH_KEY := UTF8.EncodeAscii("branchKey");
+  const CASE_A := UTF8.EncodeAscii("caseA");
+  const CASE_B := UTF8.EncodeAscii("caseB");
+  const BRANCH_KEY_ID_A := BRANCH_KEY_ID
+  const BRANCH_KEY_ID_B := ACTIVE_ACTIVE_BRANCH_KEY_ID
+
   method GetTestMaterials(suiteId: Types.AlgorithmSuiteId) returns (out: Types.EncryptionMaterials) 
   {
     var mpl :- expect MaterialProviders.MaterialProviders();
@@ -49,16 +60,33 @@ module TestAwsKmsHierarchicalKeyring {
   
   method {:test} TestHierarchyClientESDKSuite()
   {
-    var branchKeyId := "hierarchy-test-v1";
+    var branchKeyId := BRANCH_KEY_ID;
     var ttl : Types.PositiveLong := (1 * 60000) * 10;
+    var kmsClient :- expect KMS.KMSClient();
+    var mpl :- expect MaterialProviders.MaterialProviders();
+    var dynamodbClient :- expect DDB.DynamoDBClient();
+    var hierarchyKeyring :- expect mpl.CreateAwsKmsHierarchicalKeyring(
+      Types.CreateAwsKmsHierarchicalKeyringInput(
+        branchKeyId := Some(branchKeyId),
+        branchKeyIdSupplier := None,
+        kmsKeyId := keyArn,
+        kmsClient := kmsClient,
+        ddbClient := dynamodbClient,
+        branchKeyStoreArn := branchKeyStoreArn,
+        ttlSeconds := ttl,
+        maxCacheSize := Option.Some(10),
+        grantTokens := Option.None
+      )
+    );
+
     var materials := GetTestMaterials(TEST_ESDK_ALG_SUITE_ID);
-    BuildKeyringAndTestEndToEnd(materials, TEST_ESDK_ALG_SUITE_ID, branchKeyId, ttl);
+    TestRoundtrip(hierarchyKeyring, materials, TEST_ESDK_ALG_SUITE_ID, branchKeyId);
 
     //Test with key in the materials
     var suite := AlgorithmSuites.GetSuite(TEST_ESDK_ALG_SUITE_ID);
     var zeroedKey := seq(AlgorithmSuites.GetEncryptKeyLength(suite) as nat, _ => 0); // Key is Zero
     materials := materials.(plaintextDataKey := Some(zeroedKey));
-    BuildKeyringAndTestEndToEnd(materials, TEST_ESDK_ALG_SUITE_ID, branchKeyId, ttl);
+    TestRoundtrip(hierarchyKeyring, materials, TEST_ESDK_ALG_SUITE_ID, branchKeyId);
   }
 
   method {:test} TestTwoActiveKeysESDKSuite() 
@@ -67,29 +95,63 @@ module TestAwsKmsHierarchicalKeyring {
     // They have "create-time" timestamps of: 2023-03-07T17:09Z and 2023-03-07T17:07Z
     // When sorting them lexicographically, we should be using 2023-03-07T17:09Z as the "newest" 
     // branch key since this timestamp is more recent.
-    var branchKeyId := "hierarchy-test-active-active";
+    var branchKeyId := ACTIVE_ACTIVE_BRANCH_KEY_ID;
     var ttl : Types.PositiveLong := (1 * 60000) * 10;
+    var kmsClient :- expect KMS.KMSClient();
+    var mpl :- expect MaterialProviders.MaterialProviders();
+    var dynamodbClient :- expect DDB.DynamoDBClient();
+    var hierarchyKeyring :- expect mpl.CreateAwsKmsHierarchicalKeyring(
+      Types.CreateAwsKmsHierarchicalKeyringInput(
+        branchKeyId := Some(branchKeyId),
+        branchKeyIdSupplier := None,
+        kmsKeyId := keyArn,
+        kmsClient := kmsClient,
+        ddbClient := dynamodbClient,
+        branchKeyStoreArn := branchKeyStoreArn,
+        ttlSeconds := ttl,
+        maxCacheSize := Option.Some(10),
+        grantTokens := Option.None
+      )
+    );
+
     var materials := GetTestMaterials(TEST_ESDK_ALG_SUITE_ID);
-    BuildKeyringAndTestEndToEnd(materials, TEST_ESDK_ALG_SUITE_ID, branchKeyId, ttl);
+    TestRoundtrip(hierarchyKeyring, materials, TEST_ESDK_ALG_SUITE_ID, branchKeyId);
     
     //Test with key in the materials
     var suite := AlgorithmSuites.GetSuite(TEST_ESDK_ALG_SUITE_ID);
     var zeroedKey := seq(AlgorithmSuites.GetEncryptKeyLength(suite) as nat, _ => 0); // Key is Zero
     materials := materials.(plaintextDataKey := Some(zeroedKey));
-    BuildKeyringAndTestEndToEnd(materials, TEST_ESDK_ALG_SUITE_ID, branchKeyId, ttl);
+    TestRoundtrip(hierarchyKeyring, materials, TEST_ESDK_ALG_SUITE_ID, branchKeyId);
   }
 
   method {:test} TestHierarchyClientDBESuite() {
-    var branchKeyId := "hierarchy-test-v1";
+    var branchKeyId := BRANCH_KEY_ID;
     var ttl : Types.PositiveLong := (1 * 60000) * 10;
+    var kmsClient :- expect KMS.KMSClient();
+    var mpl :- expect MaterialProviders.MaterialProviders();
+    var dynamodbClient :- expect DDB.DynamoDBClient();
+    var hierarchyKeyring :- expect mpl.CreateAwsKmsHierarchicalKeyring(
+      Types.CreateAwsKmsHierarchicalKeyringInput(
+        branchKeyId := Some(branchKeyId),
+        branchKeyIdSupplier := None,
+        kmsKeyId := keyArn,
+        kmsClient := kmsClient,
+        ddbClient := dynamodbClient,
+        branchKeyStoreArn := branchKeyStoreArn,
+        ttlSeconds := ttl,
+        maxCacheSize := Option.Some(10),
+        grantTokens := Option.None
+      )
+    );
+
     var materials := GetTestMaterials(TEST_DBE_ALG_SUITE_ID);
-    BuildKeyringAndTestEndToEnd(materials, TEST_DBE_ALG_SUITE_ID, branchKeyId, ttl);
+    TestRoundtrip(hierarchyKeyring, materials, TEST_DBE_ALG_SUITE_ID, branchKeyId);
 
     //Test with key in the materials
     var suite := AlgorithmSuites.GetSuite(TEST_DBE_ALG_SUITE_ID);
     var zeroedKey := seq(AlgorithmSuites.GetEncryptKeyLength(suite) as nat, _ => 0); // Key is Zero
     materials := materials.(plaintextDataKey := Some(zeroedKey));
-    BuildKeyringAndTestEndToEnd(materials, TEST_DBE_ALG_SUITE_ID, branchKeyId, ttl);
+    TestRoundtrip(hierarchyKeyring, materials, TEST_DBE_ALG_SUITE_ID, branchKeyId);
   }
   
   method {:test} TestTwoActiveKeysDBESuite() 
@@ -98,31 +160,47 @@ module TestAwsKmsHierarchicalKeyring {
     // They have "create-time" timestamps of: 2023-03-07T17:09Z and 2023-03-07T17:07Z
     // When sorting them lexicographically, we should be using 2023-03-07T17:09Z as the "newest" 
     // branch key since this timestamp is more recent.
-    var branchKeyId := "hierarchy-test-active-active";
+    var branchKeyId := ACTIVE_ACTIVE_BRANCH_KEY_ID;
     var ttl : Types.PositiveLong := (1 * 60000) * 10;
+    var kmsClient :- expect KMS.KMSClient();
+    var mpl :- expect MaterialProviders.MaterialProviders();
+    var dynamodbClient :- expect DDB.DynamoDBClient();
+    var hierarchyKeyring :- expect mpl.CreateAwsKmsHierarchicalKeyring(
+      Types.CreateAwsKmsHierarchicalKeyringInput(
+        branchKeyId := Some(branchKeyId),
+        branchKeyIdSupplier := None,
+        kmsKeyId := keyArn,
+        kmsClient := kmsClient,
+        ddbClient := dynamodbClient,
+        branchKeyStoreArn := branchKeyStoreArn,
+        ttlSeconds := ttl,
+        maxCacheSize := Option.Some(10),
+        grantTokens := Option.None
+      )
+    );
+
     var materials := GetTestMaterials(TEST_DBE_ALG_SUITE_ID);
-    BuildKeyringAndTestEndToEnd(materials, TEST_DBE_ALG_SUITE_ID, branchKeyId, ttl);
+    TestRoundtrip(hierarchyKeyring, materials, TEST_DBE_ALG_SUITE_ID, branchKeyId);
 
     //Test with key in the materials
     var suite := AlgorithmSuites.GetSuite(TEST_DBE_ALG_SUITE_ID);
     var zeroedKey := seq(AlgorithmSuites.GetEncryptKeyLength(suite) as nat, _ => 0); // Key is Zero
     materials := materials.(plaintextDataKey := Some(zeroedKey));
-    BuildKeyringAndTestEndToEnd(materials, TEST_DBE_ALG_SUITE_ID, branchKeyId, ttl);
+    TestRoundtrip(hierarchyKeyring, materials, TEST_DBE_ALG_SUITE_ID, branchKeyId);
   }
 
-  method BuildKeyringAndTestEndToEnd(
-    encryptionMaterialsIn: Types.EncryptionMaterials,
-    algorithmSuiteId: Types.AlgorithmSuiteId,
-    branchKeyId: string,
-    ttl: Types.PositiveLong 
-  ) {
+
+  method {:test} TestBranchKeyIdSupplier() 
+  {
+    var branchKeyIdSupplier: Types.IBranchKeyIdSupplier := new DummyBranchKeyIdSupplier(); 
+    var ttl : int64 := (1 * 60000) * 10;
     var mpl :- expect MaterialProviders.MaterialProviders();
     var kmsClient :- expect KMS.KMSClient();
     var dynamodbClient :- expect DDB.DynamoDBClient();
-
-    var hierarchyKeyringResult := mpl.CreateAwsKmsHierarchicalKeyring(
+    var hierarchyKeyring :- expect mpl.CreateAwsKmsHierarchicalKeyring(
       Types.CreateAwsKmsHierarchicalKeyringInput(
-        branchKeyId := branchKeyId,
+        branchKeyId := None,
+        branchKeyIdSupplier := Some(branchKeyIdSupplier),
         kmsKeyId := keyArn,
         kmsClient := kmsClient,
         ddbClient := dynamodbClient,
@@ -133,24 +211,47 @@ module TestAwsKmsHierarchicalKeyring {
       )
     );
     
-    expect hierarchyKeyringResult.Success?;
-    var hierarchyKeyring := hierarchyKeyringResult.value;
-    
+    // Test Encryption Context with Case A
+    var materials := GetTestMaterials(TEST_DBE_ALG_SUITE_ID);
+    var contextCaseA := materials.encryptionContext[BRANCH_KEY := CASE_A];
+    materials := materials.(encryptionContext := contextCaseA);
+    TestRoundtrip(hierarchyKeyring, materials, TEST_DBE_ALG_SUITE_ID, BRANCH_KEY_ID_A); 
+
+    // Test Encryption Context with Case B
+    var contextCaseB := materials.encryptionContext[BRANCH_KEY := CASE_B];
+    materials := materials.(encryptionContext := contextCaseB);
+    TestRoundtrip(hierarchyKeyring, materials, TEST_DBE_ALG_SUITE_ID, BRANCH_KEY_ID_B); 
+  }
+
+  method TestRoundtrip(
+    hierarchyKeyring: Types.IKeyring,
+    encryptionMaterialsIn: Types.EncryptionMaterials,
+    algorithmSuiteId: Types.AlgorithmSuiteId,
+    expectedBranchKeyId: string
+  )
+    requires hierarchyKeyring.ValidState()
+    modifies hierarchyKeyring.Modifies
+    ensures hierarchyKeyring.ValidState()
+  {
     var encryptionMaterialsOut :- expect hierarchyKeyring.OnEncrypt(
       Types.OnEncryptInput(materials:=encryptionMaterialsIn)
     );
     
+    var mpl :- expect MaterialProviders.MaterialProviders();
     var _ :- expect mpl.EncryptionMaterialsHasPlaintextDataKey(encryptionMaterialsOut.materials);
 
     expect |encryptionMaterialsOut.materials.encryptedDataKeys| == 1;
 
     var edk := encryptionMaterialsOut.materials.encryptedDataKeys[0];
+    
+    // Verify the edk was created with the expected branch key
+    var expectedBranchKeyIdUTF8 :- expect UTF8.Encode(expectedBranchKeyId);
+    expect edk.keyProviderInfo == expectedBranchKeyIdUTF8;
 
-    var encryptionContext := TestUtils.SmallEncryptionContext(TestUtils.SmallEncryptionContextVariation.A);
     var decryptionMaterialsIn :- expect mpl.InitializeDecryptionMaterials(
       Types.InitializeDecryptionMaterialsInput(
         algorithmSuiteId := algorithmSuiteId,
-        encryptionContext := encryptionContext,
+        encryptionContext := encryptionMaterialsIn.encryptionContext,
         requiredEncryptionContextKeys := []
       )
     );
@@ -168,5 +269,47 @@ module TestAwsKmsHierarchicalKeyring {
     //# modified materials.
     expect encryptionMaterialsOut.materials.plaintextDataKey
     == decryptionMaterialsOut.materials.plaintextDataKey;
+  }
+
+  // Returns "hierarchy-test-v1" when EC contains kv pair "branchKey":"caseA"
+  // Returns "hierarchy-test-active-active" when EC contains kv pair "branchKey":"caseB"
+  // Otherwise returns a Failure
+  class DummyBranchKeyIdSupplier extends Types.IBranchKeyIdSupplier
+  {
+    predicate ValidState()
+      ensures ValidState() ==> History in Modifies
+    {
+      History in Modifies
+    }
+
+    constructor()
+      ensures ValidState() && fresh(this) && fresh(History) && fresh(Modifies)
+    {
+      History := new Types.IBranchKeyIdSupplierCallHistory();
+      Modifies := {History};
+    }
+
+    predicate GetBranchKeyIdEnsuresPublicly(input: Types.GetBranchKeyIdInput, output: Result<Types.GetBranchKeyIdOutput, Types.Error>)
+    {true}
+
+    method GetBranchKeyId'(input: Types.GetBranchKeyIdInput)
+        returns (output: Result<Types.GetBranchKeyIdOutput, Types.Error>)
+      requires ValidState()
+      modifies Modifies - {History}
+      decreases Modifies - {History}
+      ensures ValidState()
+      ensures GetBranchKeyIdEnsuresPublicly(input, output)
+      ensures unchanged(History)
+    {
+      var context := input.encryptionContext;
+
+      if BRANCH_KEY in context.Keys && context[BRANCH_KEY] == CASE_A {
+        return Success(Types.GetBranchKeyIdOutput(branchKeyId:=BRANCH_KEY_ID_A));
+      } else if BRANCH_KEY in context.Keys && context[BRANCH_KEY] == CASE_B {
+        return Success(Types.GetBranchKeyIdOutput(branchKeyId:=BRANCH_KEY_ID_B));
+      } else {
+        return Failure(Types.AwsCryptographicMaterialProvidersException(message := "Can't determine branchKeyId from context"));
+      }
+    }
   }
 }
